Implement mlswg/mls-protocol#720 (ciphersuite in group context)

fstar/MLS.Test.FromExt.KeySchedule.fst
@@ -13,14 +13,16 @@ open MLS.Crypto
 open MLS.TreeDEM.Keys
 open MLS.TreeDEM.PSK
 
-val gen_group_context: {|bytes_like bytes|} -> string -> nat -> keyschedule_test_epoch_input -> ML bytes
-let gen_group_context group_id epoch inp =
+val gen_group_context: {|crypto_bytes bytes|} -> string -> nat -> keyschedule_test_epoch_input -> ML bytes
+let gen_group_context #cb group_id epoch inp =
   let group_id = hex_string_to_bytes group_id in
   let tree_hash = hex_string_to_bytes inp.tree_hash in
   let confirmed_transcript_hash = hex_string_to_bytes inp.confirmed_transcript_hash in
   if length group_id < pow2 30 && epoch < (pow2 64) && length tree_hash < pow2 30 && length confirmed_transcript_hash < pow2 30 then (
     bytes_length_nil #bytes ps_extension_nt;
     (ps_to_pse ps_group_context_nt).serialize_exact ({
+      version = PV_mls10 ();
+      cipher_suite = available_ciphersuite_to_network (ciphersuite #bytes);
       group_id = group_id;
       epoch = epoch;
       tree_hash = tree_hash;
